a try with stream of memories

NLustre/MemSemantics3.v
@@ -69,150 +69,211 @@ Module Type MEMSEMANTICS
        (Import NoD   : NODUP       Ids Op       Clks Syn         Mem IsD IsV)
        (Import WeF   : WELLFORMED  Ids Op       Clks Syn     Ord Mem IsD IsV IsF NoD).
 
-  Definition memory := memory (stream val).
+  Definition memories := stream (memory val).
 
-  Definition mask'' {A} (k: nat) (rs: cstream) (xs ys: stream A) : Prop :=
-    ys 0 = xs 0
-    /\ forall n, ys n = match nat_compare (count rs n) k with
-                  | Lt => xs 0
-                  | Eq => xs (if rs n then 0 else n)
-                  | Gt => if EqNat.beq_nat (count rs n) (S k) && rs n
-                         then xs n else ys (pred n)
-                  end.
+  (* Definition mask'' {A} (k: nat) (rs: cstream) (xs ys: stream A) : Prop := *)
+  (*   ys 0 = xs 0 *)
+  (*   /\ forall n, ys n = match nat_compare (count rs n) k with *)
+  (*                 | Lt => xs 0 *)
+  (*                 | Eq => xs (if rs n then 0 else n) *)
+  (*                 | Gt => if EqNat.beq_nat (count rs n) (S k) && rs n *)
+  (*                        then xs n else ys (pred n) *)
+  (*                 end. *)
 
-  Fixpoint mask' {A} (k: nat) (rs: cstream) (xs: stream A) (n: nat) : A :=
+  (* Fixpoint mask' {A} (k: nat) (rs: cstream) (xs: stream A) (n: nat) : A := *)
+  (*   match n with *)
+  (*   | 0 => xs 0 *)
+  (*   | S n' => *)
+  (*     match nat_compare (count rs n) k with *)
+  (*     | Lt => xs 0 *)
+  (*     | Eq => xs (if rs n then 0 else n) *)
+  (*     | Gt => if EqNat.beq_nat (count rs n) (S k) && rs n *)
+  (*            then xs n else mask' k rs xs n' *)
+  (*     end *)
+  (*   end. *)
+
+  (* Lemma mask'_eq: *)
+  (*   forall {A} n k rs (xs: stream A), *)
+  (*     count rs n = k -> *)
+  (*     mask' k rs xs n = xs (if rs n then 0 else n). *)
+  (* Proof. *)
+  (*   destruct n; intros ** Count; simpl in *. *)
+  (*   - now destruct (rs 0). *)
+  (*   - apply nat_compare_eq_iff in Count; now rewrite Count. *)
+  (* Qed. *)
+
+  (* Lemma mask'_lt: *)
+  (*   forall {A} n k rs (xs: stream A), *)
+  (*     count rs n < k -> *)
+  (*     mask' k rs xs n = xs 0. *)
+  (* Proof. *)
+  (*   destruct n; intros ** Count; simpl in *; auto. *)
+  (*   apply nat_compare_lt in Count; now rewrite Count. *)
+  (* Qed. *)
+
+  (* Lemma mask'_spec: *)
+  (*   forall {A} k rs (xs: stream A), *)
+  (*     mask'' k rs xs (mask' k rs xs). *)
+  (* Proof. *)
+  (*   split; auto. *)
+  (*   induction n; simpl; auto. *)
+  (*   destruct (nat_compare (if rs 0 then 1 else 0) k), (rs 0); simpl; auto. *)
+  (*   destruct k; simpl; auto. *)
+  (* Qed. *)
+
+  Fixpoint mmask (k: nat) (rs: cstream) (M: memories) (n: nat) : memory val :=
     match n with
-    | 0 => xs 0
-    | S n' =>
-      match nat_compare (count rs n) k with
-      | Lt => xs 0
-      | Eq => xs (if rs n then 0 else n)
-      | Gt => if EqNat.beq_nat (count rs n) (S k) && rs n
-             then xs n else mask' k rs xs n'
-      end
+    | 0 => M 0
+    | S n' => match nat_compare (count rs n) k with
+             | Lt => M 0
+             | Eq => M (if rs n then 0 else n)
+             | Gt => if EqNat.beq_nat (count rs n) (S k) && rs n
+                    then M n else mmask k rs M n'
+             end
     end.
 
-  Lemma mask'_eq:
-    forall {A} n k rs (xs: stream A),
+  (* Lemma mmask_mfind_mem: *)
+  (*   forall x M n k rs, *)
+  (*     mfind_mem x (M n) <> None -> *)
+  (*     mfind_mem x (mmask k rs M n) <> None. *)
+  (* Proof. *)
+  (*   intros ** E E'; apply E; clear E. *)
+  (*   induction n; simpl in *; auto. *)
+  (*   destruct () *)
+  (*   - contradiction. *)
+
+
+  Lemma mmask_eq:
+    forall n k rs M,
       count rs n = k ->
-      mask' k rs xs n = xs (if rs n then 0 else n).
+      mmask k rs M n = M (if rs n then 0 else n).
   Proof.
     destruct n; intros ** Count; simpl in *.
     - now destruct (rs 0).
     - apply nat_compare_eq_iff in Count; now rewrite Count.
   Qed.
 
-  Lemma mask'_lt:
-    forall {A} n k rs (xs: stream A),
+  Lemma mmask_lt:
+    forall n k rs M,
       count rs n < k ->
-      mask' k rs xs n = xs 0.
+      mmask k rs M n = M 0.
   Proof.
     destruct n; intros ** Count; simpl in *; auto.
     apply nat_compare_lt in Count; now rewrite Count.
   Qed.
 
-  Lemma mask'_spec:
-    forall {A} k rs (xs: stream A),
-      mask'' k rs xs (mask' k rs xs).
+  Lemma mmask_gt:
+    forall n k rs M,
+      count rs (S n) > k ->
+      mmask k rs M (S n) = if EqNat.beq_nat (count rs (S n)) (S k) && rs (S n)
+                           then M (S n) else mmask k rs M n.
   Proof.
-    split; auto.
-    induction n; simpl; auto.
-    destruct (nat_compare (if rs 0 then 1 else 0) k), (rs 0); simpl; auto.
-    destruct k; simpl; auto.
+    intros ** Count; simpl in *.
+    apply nat_compare_gt in Count; now rewrite Count.
   Qed.
 
-  Definition mmask' (k: nat) (rs: cstream) (M M': memory) : Prop :=
-    forall x ms,
-      mfind_mem x M = Some ms ->
-      mfind_mem x M' = Some (mask' k rs ms).
 
-  Definition mmask (k: nat) (rs: cstream) (M: memory) : memory :=
-    mmap (mask' k rs) M.
-  (* Definition mflatten (Ms: nat -> memory) (M: memory) : Prop := *)
-  (*   forall k, Ms k *)
 
-  Definition memory_reset (rs: cstream) (M: memory) : memory :=
-    mmap (fun ms => fun n => ms (if rs n then 0 else n)) M.
+  (* Definition memory_reset (rs: cstream) (M: memory) : memory := *)
+  (*   mmap (fun ms => fun n => ms (if rs n then 0 else n)) M. *)
 
-  Inductive mfby: ident -> val -> stream value -> memory -> stream value -> Prop :=
+  Inductive mfby: ident -> val -> stream value -> memories -> stream value -> Prop :=
     mfby_intro:
-      forall x v0 ls M xs ms,
-        mfind_mem x M = Some ms ->
-        ms 0 = v0 ->
-        (forall n, match ls n with
-              | absent    => ms (S n) = ms n /\ xs n = absent
-              | present v => ms (S n) = v    /\ xs n = present (ms n)
+      forall x v0 ls M xs,
+        mfind_mem x (M 0) = Some v0 ->
+        (forall n, match mfind_mem x (M n) with
+              | Some mv =>
+                match ls n with
+                | absent    => mfind_mem x (M (S n)) = Some mv /\ xs n = absent
+                | present v => mfind_mem x (M (S n)) = Some v  /\ xs n = present mv
+                end
+              | None => False
               end) ->
         mfby x v0 ls M xs.
+
+  Lemma mmask_mfby:
+    forall M x v0 xs ls k rs n,
+      mfby x v0 ls M xs ->
+      mfind_mem x (mmask k rs M n) <> None.
+  Proof.
+    intros ** Fby Find'; inversion_clear Fby as [????? Find Spec].
+    induction n; simpl in Find'.
+    - rewrite Find in Find'; discriminate.
+    - destruct (nat_compare (if rs (S n) then S (count rs n) else count rs n) k), (rs (S n));
+        try (now rewrite Find in Find'; discriminate).
+      + specialize (Spec (S n)); rewrite Find' in Spec; auto.
+      + destruct (EqNat.beq_nat (S (count rs n)) (S k) && true); auto.
+        specialize (Spec (S n)); rewrite Find' in Spec; auto.
+      + destruct (EqNat.beq_nat (count rs n) (S k) && false); auto.
+        specialize (Spec (S n)); rewrite Find' in Spec; auto.
+  Qed.
 
   Lemma foo:
     forall x v0 ls M xs k rs,
       mfby x v0 ls M xs ->
-      (forall ms,
-          mfind_mem x M = Some ms ->
-          forall n,
-            rs n = true ->
-            ms n = v0) ->
+      (forall n,
+          rs n = true ->
+          mfind_mem x (M n) = Some v0) ->
       mfby x v0 (mask absent k rs ls) (mmask k rs M) (mask absent k rs xs).
   Proof.
     intros ** Fby Rst.
-    inversion_clear Fby as [?????? Find ? Spec].
-    specialize (Rst _ Find).
-    (* apply Mask in Find. *)
-    econstructor.
-    - apply mfind_mem_map; eauto.
-    - auto.
-    - intro n; specialize (Spec n); specialize (Rst n).
-      unfold mask; simpl.
-      destruct (nat_compare (count rs n) k) eqn: E.
-      + assert (EqNat.beq_nat k (count rs n) = true) as ->
-            by now rewrite NPeano.Nat.eqb_sym, EqNat.beq_nat_true_iff,
-               <-nat_compare_eq_iff.
-        rewrite mask'_eq by now apply nat_compare_eq_iff.
-        destruct (rs (S n)).
-        *{ assert (nat_compare (S (count rs n)) k = Gt) as ->
-               by (rewrite <-nat_compare_gt; apply Gt.le_gt_S;
-                   apply nat_compare_eq_iff in E; omega).
-           assert (EqNat.beq_nat (S (count rs n)) (S k) = true) as ->
-               by now apply EqNat.beq_nat_true_iff, eq_sym,
-                  eq_S, EqNat.beq_nat_true_iff.
-           destruct (ls n), (rs n); simpl; intuition; rewrite H.
-           - now rewrite H3.
-           - now rewrite <-H5.
-         }
-        *{ rewrite E.
-           destruct (ls n), (rs n); intuition; rewrite H.
-           - now rewrite H1.
-           - now rewrite <-H3.
-         }
-      + assert (EqNat.beq_nat k (count rs n) = false) as ->
-            by (apply nat_compare_lt in E; apply EqNat.beq_nat_false_iff;
-                intro; subst; omega).
-        rewrite mask'_lt by now apply nat_compare_lt.
-        destruct (rs (S n)).
-        * destruct (nat_compare (S (count rs n)) k) eqn: E'; intuition.
-          apply nat_compare_lt in E; apply nat_compare_gt in E'; omega.
-        * now rewrite E.
-      + assert (EqNat.beq_nat k (count rs n) = false) as ->
-            by (apply nat_compare_gt in E; apply EqNat.beq_nat_false_iff;
-                intro; subst; omega).
-        destruct (rs (S n)).
-        * assert (nat_compare (S (count rs n)) k = Gt) as ->
-              by (rewrite <-nat_compare_gt in *; omega).
-          assert (EqNat.beq_nat (S (count rs n)) (S k) = false) as ->
-              by now apply EqNat.beq_nat_false_iff, not_eq_S,
-                 not_eq_sym, EqNat.beq_nat_false_iff.
-          now rewrite Bool.andb_false_l.
-        * now rewrite E, Bool.andb_false_r.
+    inversion_clear Fby as [????? Find Spec].
+    econstructor; eauto.
+    intro n(* ; specialize (Spec n); specialize (Rst n) *).
+    unfold mask; simpl.
+    destruct (nat_compare (count rs n) k) eqn: E.
+    - specialize (Spec n); specialize (Rst n).
+      assert (EqNat.beq_nat k (count rs n) = true) as ->
+          by now rewrite NPeano.Nat.eqb_sym, EqNat.beq_nat_true_iff,
+             <-nat_compare_eq_iff.
+      rewrite mmask_eq by now apply nat_compare_eq_iff.
+      destruct (rs (S n)).
+      + assert (nat_compare (S (count rs n)) k = Gt) as ->
+            by (rewrite <-nat_compare_gt; apply Gt.le_gt_S;
+                apply nat_compare_eq_iff in E; omega).
+        assert (EqNat.beq_nat (S (count rs n)) (S k) = true) as ->
+            by now apply EqNat.beq_nat_true_iff, eq_sym,
+               eq_S, EqNat.beq_nat_true_iff.
+        destruct (ls n), (rs n); simpl; intuition;
+          rewrite H2 in Spec; rewrite Find; intuition.
+      + rewrite E.
+        destruct (ls n), (rs n); intuition;
+          rewrite H0 in Spec; rewrite Find; intuition.
+    - assert (EqNat.beq_nat k (count rs n) = false) as ->
+          by (apply nat_compare_lt in E; apply EqNat.beq_nat_false_iff;
+              intro; subst; omega).
+      rewrite mmask_lt by (now apply nat_compare_lt); rewrite Find.
+      destruct (rs (S n)).
+      + destruct (nat_compare (S (count rs n)) k) eqn: E'; intuition.
+        apply nat_compare_lt in E; apply nat_compare_gt in E'; omega.
+      + rewrite E; auto.
+    - assert (EqNat.beq_nat k (count rs n) = false) as ->
+          by (apply nat_compare_gt in E; apply EqNat.beq_nat_false_iff;
+              intro; subst; omega).
+      destruct (rs (S n)).
+      + assert (nat_compare (S (count rs n)) k = Gt) as ->
+            by (rewrite <-nat_compare_gt in *; omega).
+        assert (EqNat.beq_nat (S (count rs n)) (S k) = false) as ->
+            by (apply EqNat.beq_nat_false_iff, not_eq_S,
+                not_eq_sym; apply nat_compare_gt in E; omega).
+        simpl.
+        destruct (mfind_mem x (mmask k rs M n)) eqn: Find'; auto.
+        eapply mmask_mfby; eauto using mfby.
+      + rewrite E, Bool.andb_false_r.
+        destruct (mfind_mem x (mmask k rs M n)) eqn: Find'; auto.
+        eapply mmask_mfby; eauto using mfby.
   Qed.
 
-  Implicit Type M : memory.
+  (* Implicit Type M : memory. *)
 
   Section NodeSemantics.
 
+    Definition sub_inst (x: ident) (M M': memories) : Prop :=
+      forall n, mfind_inst x (M n) = Some (M' n).
+
     Variable G: global.
 
-    Inductive msem_equation: stream bool -> history -> memory -> equation -> Prop :=
+    Inductive msem_equation: stream bool -> history -> memories -> equation -> Prop :=
     | SEqDef:
         forall bk H M x ck xs ce,
           sem_var bk H x xs ->
@@ -221,7 +282,7 @@ Module Type MEMSEMANTICS
     | SEqApp:
         forall bk H M x xs ck f M' arg ls xss,
           Some x = hd_error xs ->
-          mfind_inst x M = Some M' ->
+          sub_inst x M M' ->
           sem_laexps bk H ck arg ls ->
           sem_vars bk H xs xss ->
           msem_node f ls M' xss ->
@@ -229,7 +290,7 @@ Module Type MEMSEMANTICS
     | SEqReset:
         forall bk H M x xs ck f M' arg y ck_r ys ls xss,
           Some x = hd_error xs ->
-          mfind_inst x M = Some M' ->
+          sub_inst x M M' ->
           sem_laexps bk H ck arg ls ->
           sem_vars bk H xs xss ->
           sem_var bk H y ys ->
@@ -243,7 +304,7 @@ Module Type MEMSEMANTICS
           msem_equation bk H M (EqFby x ck c0 le)
 
     with msem_reset:
-           ident -> stream bool -> stream (list value) -> memory ->
+           ident -> stream bool -> stream (list value) -> memories ->
            stream (list value) -> Prop :=
          | SReset:
              forall f r xss M yss,
@@ -254,7 +315,7 @@ Module Type MEMSEMANTICS
                msem_reset f r xss M yss
 
     with msem_node:
-           ident -> stream (list value) -> memory -> stream (list value) -> Prop :=
+           ident -> stream (list value) -> memories -> stream (list value) -> Prop :=
          | SNode:
              forall bk H f xss M yss n,
                clock_of xss bk ->
@@ -281,9 +342,9 @@ enough: it does not support the internal fixpoint introduced by
 
     Variable G: global.
 
-    Variable P_equation: stream bool -> history -> memory -> equation -> Prop.
-    Variable P_reset: ident -> stream bool -> stream (list value) -> memory -> stream (list value) -> Prop.
-    Variable P_node: ident -> stream (list value) -> memory -> stream (list value) -> Prop.
+    Variable P_equation: stream bool -> history -> memories -> equation -> Prop.
+    Variable P_reset: ident -> stream bool -> stream (list value) -> memories -> stream (list value) -> Prop.
+    Variable P_node: ident -> stream (list value) -> memories -> stream (list value) -> Prop.
 
     Hypothesis EqDefCase:
       forall bk H M x ck xs ce,
@@ -294,7 +355,7 @@ enough: it does not support the internal fixpoint introduced by
     Hypothesis EqAppCase:
       forall bk H M x xs ck f M' arg ls xss,
         Some x = hd_error xs ->
-        mfind_inst x M = Some M' ->
+        sub_inst x M M' ->
         sem_laexps bk H ck arg ls ->
         sem_vars bk H xs xss ->
         msem_node G f ls M' xss ->
@@ -304,7 +365,7 @@ enough: it does not support the internal fixpoint introduced by
     Hypothesis EqResetCase:
       forall bk H M x xs ck f M' arg y ck_r ys ls xss,
         Some x = hd_error xs ->
-        mfind_inst x M = Some M' ->
+        sub_inst x M M' ->
         sem_laexps bk H ck arg ls ->
         sem_vars bk H xs xss ->
         sem_var bk H y ys ->
@@ -345,20 +406,20 @@ enough: it does not support the internal fixpoint introduced by
         P_node f xss M yss.
 
     Fixpoint msem_equation_mult
-             (b: stream bool) (H: history) (M: memory) (e: equation)
+             (b: stream bool) (H: history) (M: memories) (e: equation)
              (Sem: msem_equation G b H M e) {struct Sem}
       : P_equation b H M e
     with msem_reset_mult
            (f: ident) (r: stream bool)
            (xss: stream (list value))
-           (M: memory)
+           (M: memories)
            (oss: stream (list value))
            (Sem: msem_reset G f r xss M oss) {struct Sem}
          : P_reset f r xss M oss
     with msem_node_mult
            (f: ident)
            (xss: stream (list value))
-           (M: memory)
+           (M: memories)
            (oss: stream (list value))
            (Sem: msem_node G f xss M oss) {struct Sem}
          : P_node f xss M oss.
@@ -648,31 +709,41 @@ enough: it does not support the internal fixpoint introduced by
 
   (** *** Memory management *)
 
-  Lemma mfby_madd_mem:
+  Definition add_mems (y: ident) (ms: stream val) (M: memories): memories :=
+    fun n => madd_mem y (ms n) (M n).
+
+  Lemma mfby_add_mems:
     forall x v0 ls M xs y ms,
       x <> y ->
       mfby x v0 ls M xs ->
-      mfby x v0 ls (madd_mem y ms M) xs.
+      mfby x v0 ls (add_mems y ms M) xs.
   Proof.
-    inversion 2; econstructor; eauto.
-    rewrite mfind_mem_gso; auto.
+    unfold add_mems.
+    intros ** Fby; inversion_clear Fby as [?????? Spec].
+    constructor.
+    - rewrite mfind_mem_gso; auto.
+    - intro n; rewrite 2 mfind_mem_gso; auto.
+      exact (Spec n).
   Qed.
 
-  Lemma mfby_madd_obj:
+  Definition add_objs (y: ident) (M' M: memories): memories :=
+    fun n => madd_obj y (M' n) (M n).
+
+  Lemma mfby_add_objs:
     forall x v0 ls M xs y M',
       mfby x v0 ls M xs ->
-      mfby x v0 ls (madd_obj y M' M) xs.
+      mfby x v0 ls (add_objs y M' M) xs.
   Proof.
     inversion 1; econstructor; eauto.
   Qed.
 
-  Hint Resolve mfby_madd_mem mfby_madd_obj.
+  Hint Resolve mfby_add_mems mfby_add_objs.
 
   Lemma msem_equation_madd_mem:
     forall G bk H M x ms eqs,
       ~Is_defined_in_eqs x eqs ->
       Forall (msem_equation G bk H M) eqs ->
-      Forall (msem_equation G bk H (madd_mem x ms M)) eqs.
+      Forall (msem_equation G bk H (add_mems x ms M)) eqs.
   Proof.
     Hint Constructors msem_equation.
     intros ** Hnd Hsem.
@@ -691,7 +762,7 @@ enough: it does not support the internal fixpoint introduced by
     forall G bk H M M' x eqs,
       ~Is_defined_in_eqs x eqs ->
       Forall (msem_equation G bk H M) eqs ->
-      Forall (msem_equation G bk H (madd_obj x M' M)) eqs.
+      Forall (msem_equation G bk H (add_objs x M' M)) eqs.
   Proof.
     Hint Constructors msem_equation.
     intros * Hnd Hsem.
@@ -704,9 +775,9 @@ enough: it does not support the internal fixpoint introduced by
     destruct Hsem as [|? ? ? x' ? ? ? ? ? ? ? Hsome
                          |? ? ? x' ? ? ? ? ? ? ? ? ? ? Hsome|];
       eauto;
-      assert (mfind_inst x' (madd_obj x M' M) = Some M'0)
+      assert (sub_inst x' (add_objs x M' M) M'0)
         by (apply not_Is_defined_in_eq_EqApp in Hnd;
-            rewrite mfind_inst_gso; auto;
+            unfold sub_inst, add_objs; intro; rewrite mfind_inst_gso; auto;
             intro; subst x; destruct xs; inv Hsome; apply Hnd; now constructor);
       eauto.
   Qed.
@@ -773,7 +844,7 @@ dataflow memory for which the non-standard semantics holds true.
     - exists M.
       repeat (econstructor; eauto).
     - apply IH in Hsem as [M' Hmsem].
-      exists (madd_obj (hd Ids.default x) M' M).
+      exists (add_objs (hd Ids.default x) M' M).
 
       assert (exists i, Some i = hd_error x) as [i Hsome].
       {
@@ -810,7 +881,7 @@ dataflow memory for which the non-standard semantics holds true.
 
       constructor.
       + econstructor; eauto.
-        now apply mfind_inst_gss.
+        unfold sub_inst, add_objs; intro; now apply mfind_inst_gss.
       + inversion_clear Hwsch.
         assert (Is_defined_in_eq i (EqApp x ck f arg None)).
         {
@@ -821,7 +892,7 @@ dataflow memory for which the non-standard semantics holds true.
 
     - pose proof Hsem as Hsem'.
       apply IH' in Hsem as [M' Hmsem].
-      exists (madd_obj (hd Ids.default x) M' M).
+      exists (add_objs (hd Ids.default x) M' M).
 
       assert (exists i, Some i = hd_error x) as [i Hsome].
       {
@@ -866,7 +937,7 @@ dataflow memory for which the non-standard semantics holds true.
 
       constructor.
       + econstructor; eauto.
-        now apply mfind_inst_gss.
+        unfold sub_inst, add_objs; intro. now apply mfind_inst_gss.
       + inversion_clear Hwsch.
         assert (Is_defined_in_eq i (EqApp x ck f arg (Some (y, ck_r)))).
         {
@@ -875,13 +946,15 @@ dataflow memory for which the non-standard semantics holds true.
         }
         apply msem_equation_madd_obj; auto.
 
-    - exists (madd_mem x (hold (sem_const c0) ls) M).
+    - exists (add_mems x (hold (sem_const c0) ls) M).
       constructor.
-      + do 2 (econstructor; eauto).
+      + unfold add_mems.
+        do 2 (econstructor; eauto).
         * now apply mfind_mem_gss.
-        * reflexivity.
+        (* * reflexivity. *)
         * rewrite H1; unfold fby; simpl.
-          intro n; destruct (ls n); auto.
+          intro n; destruct (ls n); auto;
+            repeat rewrite mfind_mem_gss; auto.
       + inversion_clear Hwsch.
         apply msem_equation_madd_mem; eauto.
   Qed.
@@ -901,13 +974,15 @@ dataflow memory for which the non-standard semantics holds true.
       exists M', Forall (msem_equation G bk H M') eqs.
   Proof.
     intros ** IH Hwsch Heqs.
-    induction eqs as [|eq eqs IHeqs]; [exists (empty_memory _); now constructor|].
+    induction eqs as [|eq eqs IHeqs]; [exists (fun n => empty_memory _); now constructor|].
     apply Forall_cons2 in Heqs as [Heq Heqs].
     eapply IHeqs with (1:=Is_well_sch_cons _ _ _ _ Hwsch)
       in Heqs
       as [M Heqs]; eauto.
     eapply sem_msem_eq; eauto.
   Qed.
+
+  Require Import Coq.Logic.ClassicalChoice.
 
   Theorem sem_msem_node:
     forall G f xs ys,
@@ -940,11 +1015,59 @@ dataflow memory for which the non-standard semantics holds true.
       { clear - IHG'.
         intros ** Sem.
         inversion_clear Sem as [???? Sem'].
-        assert (forall n, exists M, msem_node G f (mask (all_absent (xs 0)) n r xs) M (mask (all_absent (ys 0)) n r ys))
-          by (intro; specialize (Sem' n); apply IHG' in Sem'; auto).
+        assert (forall n, exists M, msem_node G f (mask (all_absent (xs 0)) n r xs) M
+                                    (mask (all_absent (ys 0)) n r ys)) as Msem
+            by (intro; specialize (Sem' n); apply IHG' in Sem'; auto).
+        apply choice in Msem as (F & Msem).
+        assert (forall k k', F k 0 = F k' 0) as Init by admit.
+        exists (fun n => F (count r n) n).
+        constructor.
+        intro k; specialize (Msem k).
+        assert (forall n, mmask k r (fun n : nat => F (count r n) n) n = F k n).
+        { induction n; simpl.
+          - apply Init.
+          - rewrite IHn.
+            destruct (nat_compare (count r n) k) eqn: E.
+            + destruct (r (S n)) eqn: R.
+              * assert (nat_compare (S (count r n)) k = Gt) as ->
+                  by (rewrite <-nat_compare_gt; apply Gt.le_gt_S;
+                      apply nat_compare_eq_iff in E; omega).
+                assert (EqNat.beq_nat (S (count r n)) (S k) = true) as ->
+                    by now apply EqNat.beq_nat_true_iff, eq_S, nat_compare_eq.
+                simpl.
+                apply nat_compare_eq_iff in E; rewrite E.
+                admit.
+              * simpl; rewrite E, R.
+                now apply nat_compare_eq_iff in E; rewrite E.
+            + destruct (r (S n)) eqn: R.
+              *{ destruct (nat_compare (S (count r n)) k) eqn: E'.
+                 - admit.
+                 - admit.
+                 - apply nat_compare_lt in E; apply nat_compare_gt in E'; omega.
+               }
+              * rewrite E.
+                admit.
+            + destruct (r (S n)) eqn: R.
+              * assert (nat_compare (S (count r n)) k = Gt) as ->
+                    by (rewrite <-nat_compare_gt in *; omega).
+                assert (EqNat.beq_nat (S (count r n)) (S k) = false) as ->
+                    by (apply EqNat.beq_nat_false_iff, not_eq_S,
+                        not_eq_sym; apply nat_compare_gt in E; omega).
+                simpl.
+                admit.
+              * rewrite E, Bool.andb_false_r.
+                admit.
+        }
+        admit.
+        (* inversion_clear Msem as [?????????????? Heqs]. *)
+        (* econstructor; eauto. *)
+        (* induction (n_eqs n) as [|e]; auto. *)
+        (* inv Heqs; constructor; auto. *)
+        (* induction e. *)
+
+
         (* eexists. *)
         (* constructor. *)
-        admit.
       }
       inversion_clear Hwdef as [|??? neqs].
       simpl in neqs; unfold neqs in *.
@@ -956,9 +1079,9 @@ dataflow memory for which the non-standard semantics holds true.
       + eapply msem_equation_cons2; eauto.
     - apply ident_eqb_neq in Hnf.
       apply sem_node_cons with (1:=Hord) (3:=Hnf) in Hsem.
+      inv Hord.
       eapply IHG in Hsem as [M]; eauto.
       exists M.
-      inv Hord.
       now eapply msem_node_cons2; eauto.
   Qed.
 
